Day9 part 1 and 2 🎉

AoC-Lean/AoC2023/Day9.lean
@@ -3,6 +3,7 @@ import Util
 namespace Day9
 
 def Sequence := List Int
+deriving ToString
 
 def Sequence.derive : Sequence -> Sequence
   | [] => []
@@ -12,7 +13,8 @@ def Sequence.derive : Sequence -> Sequence
 
 notation "dx" s => Sequence.derive s
 
-theorem seq_len_less (seq : Sequence) : List.length (dx seq) < List.length seq := by
+theorem seq_len_less (seq : Sequence) :
+  (List.length seq > 0) → List.length (dx seq) < List.length seq := by
   sorry
 
 def allZeros : Sequence -> Bool
@@ -29,23 +31,38 @@ partial def findNext : Sequence -> Int := fun seq =>
       seq.getLast! + n
   fold seq
 
+partial def findPrevious : Sequence → Int := fun seq =>
+  let rec fold : Sequence → Int := fun seq =>
+    if allZeros seq then
+      0
+    else
+      let seq' := dx seq
+      let n := fold seq'
+      seq.head! - n
+  fold seq
+
 def parseLines : List String -> List Sequence
   | [] => []
-  | s :: ss => Util.parseInts s :: parseLines ss
+  | s :: ss =>
+    let nums := String.splitOn s " "
+    let foo := List.foldl (fun acc s => match String.toInt? s with | none => acc | some k => acc ++ [k]) [] nums
+    let rest := parseLines ss
+    foo :: rest
 
 def input : List Sequence :=
 [
   [0, 3, 6, 9, 12, 15],
   [1, 3, 6, 10, 15, 21],
-  [10, 13, 16, 21, 30, 45]
+  [10, 13, 16, 21, 30, 45],
+  [-1,-2,-3]
 ]
 
-#eval List.map findNext input
+#eval List.map findPrevious input
 
 def runDay : List String → String := fun lns =>
   let seqs := parseLines lns
-  let sln1 := Util.sum 0 (List.map findNext seqs)
-  let sln2 := 0
+  let sln1 := Util.sum (0 : Int) (List.map findNext seqs)
+  let sln2 := Util.sum (0 : Int) (List.map findPrevious seqs)
   s!"Part 1: {sln1}\nPart 2: {sln2}"
 
 end Day9
